[IsaSAT]first rescaling version

Weidenbach_Book/IsaSAT/Pairing_Heaps_Impl_LLVM.thy
@@ -2,14 +2,14 @@ theory Pairing_Heaps_Impl_LLVM
   imports Pairing_Heap_LLVM.Pairing_Heaps_Impl IsaSAT_Literals_LLVM
 begin
 
-type_synonym hp_assn = \<open>32 word ptr \<times> 32 word ptr \<times> 32 word ptr \<times> 32 word ptr \<times> 64 word ptr \<times> 32 word\<close>
+type_synonym hp_assn = \<open>32 word ptr \<times> 32 word ptr \<times> 32 word ptr \<times> 32 word ptr \<times> (64 word \<times> 64 word ptr) \<times> 32 word\<close>
 
 definition hp_assn :: \<open>_ \<Rightarrow> hp_assn \<Rightarrow> assn\<close> where
   \<open>hp_assn \<equiv> (IICF_Array.array_assn atom.option_assn \<times>\<^sub>a
     IICF_Array.array_assn atom.option_assn \<times>\<^sub>a
     IICF_Array.array_assn atom.option_assn \<times>\<^sub>a
     IICF_Array.array_assn atom.option_assn \<times>\<^sub>a
-    IICF_Array.array_assn uint64_nat_assn \<times>\<^sub>a atom.option_assn)\<close>
+    larray64_assn uint64_nat_assn \<times>\<^sub>a atom.option_assn)\<close>
 
 sepref_def mop_hp_read_prev_imp_code
   is \<open>uncurry mop_hp_read_prev_imp\<close>
@@ -322,8 +322,62 @@ lemma mop_hp_read_score_imp_mop_hp_read_score2:
   by (intro frefI nres_relI)
    (auto intro!: mop_hp_read_score_imp_mop_hp_read_score[THEN order_trans])
 
+definition mop_imp_needs_rescaling 
+  :: \<open>('a,'b)pairing_heaps_imp \<Rightarrow> nat \<Rightarrow> bool nres\<close> where
+  \<open>mop_imp_needs_rescaling = (\<lambda>_ m. 
+   RETURN (m > 1152921504606846976))\<close>
 
-thm mop_hp_read_score_imp_mop_hp_read_score
+sepref_def mop_imp_needs_rescaling_code
+  is \<open>uncurry mop_imp_needs_rescaling\<close>
+  :: \<open>(hp_assn)\<^sup>k  *\<^sub>a  uint64_nat_assn\<^sup>k \<rightarrow>\<^sub>a bool1_assn\<close>
+  unfolding mop_imp_needs_rescaling_def
+  apply (annot_unat_const \<open>TYPE(64)\<close>)
+  by sepref
+
+lemma mop_imp_needs_rescaling_mop_hp_needs_rescaling:
+  \<open>(uncurry Pairing_Heaps_Impl_LLVM.mop_imp_needs_rescaling,
+   uncurry Pairing_Heaps_Impl.mop_imp_needs_rescaling) \<in> Id \<times>\<^sub>f Id \<rightarrow>\<^sub>f \<langle>bool_rel\<rangle>nres_rel \<close>
+  unfolding mop_imp_needs_rescaling_def Pairing_Heaps_Impl.mop_hp_needs_rescaling_def
+   Pairing_Heaps_Impl.mop_imp_needs_rescaling_def
+  by (auto intro!: nres_relI frefI)
+
+
+definition mop_hp_needs_rescaling2 :: \<open>(nat multiset \<times> (nat,'c) hp_fun \<times> nat option) \<Rightarrow> nat  \<Rightarrow> bool nres\<close> where
+  \<open>mop_hp_needs_rescaling2 = (\<lambda>(\<V>, (prevs, nxts, childs, parents, scores), h) m. SPEC (\<lambda>_. True))\<close>
+
+lemma mop_imp_needs_rescaling_mop_hp_needs_rescaling2:
+  \<open>(uncurry Pairing_Heaps_Impl_LLVM.mop_imp_needs_rescaling, uncurry mop_hp_needs_rescaling2)
+    \<in> \<langle>\<langle>nat_rel\<rangle>option_rel,\<langle>nat_rel\<rangle>option_rel\<rangle>pairing_heaps_rel \<times>\<^sub>f nat_rel  \<rightarrow>\<^sub>f \<langle>bool_rel\<rangle>nres_rel\<close>
+  unfolding mop_imp_needs_rescaling_def Pairing_Heaps_Impl.mop_hp_needs_rescaling_def
+   mop_hp_needs_rescaling2_def
+  by (auto intro!: nres_relI frefI)
+
+lemmas [sepref_fr_rules] =
+  mop_imp_needs_rescaling_code.refine[FCOMP mop_imp_needs_rescaling_mop_hp_needs_rescaling2, unfolded hp_assn_def]
+
+sepref_register Pairing_Heaps_Impl.mop_imp_needs_rescaling
+
+sepref_def mop_imp_decreases_weights_pure_rescale_code
+  is \<open>uncurry mop_imp_decreases_weights_only\<close>
+  :: \<open>uint64_nat_assn\<^sup>k *\<^sub>a (hp_assn)\<^sup>d \<rightarrow>\<^sub>a hp_assn\<close>
+  supply [[goals_limit=1]]
+  supply [sepref_fr_rules] = mop_imp_needs_rescaling_code.refine[FCOMP mop_imp_needs_rescaling_mop_hp_needs_rescaling]
+  unfolding mop_imp_decreases_weights_only_def mop_hp_needs_rescaling_def[symmetric]
+    hp_assn_def
+  apply (annot_snat_const \<open>TYPE(64)\<close>)
+  by sepref
+
+thm  mop_imp_needs_rescaling_code.refine[FCOMP mop_imp_needs_rescaling_mop_hp_needs_rescaling]
+
+sepref_def mop_imp_decrease_weights_code
+  is \<open>uncurry mop_imp_decreases_weights\<close>
+  :: \<open>uint64_nat_assn\<^sup>k *\<^sub>a (hp_assn)\<^sup>d \<rightarrow>\<^sub>a hp_assn\<close>
+  supply [[goals_limit=1]]
+  supply [sepref_fr_rules] = mop_imp_needs_rescaling_code.refine[FCOMP mop_imp_needs_rescaling_mop_hp_needs_rescaling]
+  unfolding mop_imp_decreases_weights_def mop_hp_needs_rescaling_def[symmetric]
+  by sepref
+
+
 definition acids_assn :: \<open>_\<close> where
   \<open>acids_assn = hr_comp (hr_comp hp_assn (\<langle>\<langle>nat_rel\<rangle>option_rel, \<langle>nat_rel\<rangle>option_rel\<rangle>pairing_heaps_rel))
               acids_encoded_hmrel\<close>
@@ -333,11 +387,147 @@ lemmas [fcomp_norm_unfold] = acids_assn_def[symmetric]
 sepref_register ACIDS.mop_prio_change_weight ACIDS.mop_prio_insert
   ACIDS.mop_prio_pop_min ACIDS.mop_prio_is_in
 
+lemma mop_prio_change_all_weights_alt_def:
+  "ACIDS.mop_prio_change_all_weights \<equiv>  (\<lambda>(\<A>, b, w). RES {(\<A>, b,w) |w. True})"
+  unfolding ACIDS.mop_prio_change_all_weights_def bind_RES_RETURN_eq
+  by auto
+
+
+lemma hp_node_hp_rescale[simp]:
+  \<open>hp_node v (hp_rescale_weight a xx) =  map_option (hp_rescale_weight a) (hp_node v xx)\<close>
+  apply (induction v xx rule: hp_node.induct)
+  subgoal
+    by (auto split: option.splits simp: hp_node.simps simp del: hp_node_children_simps2 dest: distinct_mset_union)
+  subgoal
+    by (auto split: option.splits simp: hp_node.simps simp del: hp_node_children_simps2 dest: distinct_mset_union)
+  done
+
+lemma [simp]: \<open>map_option node (hp_next x (hp_rescale_weight x1 y)) = map_option node (hp_next x y)\<close>
+  apply (induction x y rule: hp_next.induct)
+  subgoal
+    apply (auto simp: hp_next.simps simp del: )
+    by (metis (no_types, lifting) ext hp.exhaust_sel hp.sel(1) hp_next_children_simps(1,2,3) hp_rescale_weight.simps option.map(2) option.map_disc_iff)
+  subgoal by auto
+  subgoal by auto
+  done
+
+lemma node_hp_rescale_weight[simp]: \<open>node (hp_rescale_weight x1 b) = node b\<close>
+  by (cases b) auto
+
+lemma [simp]: \<open>map_option node (hp_prev x (hp_rescale_weight x1 y)) = map_option node (hp_prev x y)\<close>
+  apply (induction x y rule: hp_prev.induct)
+  subgoal
+    by (auto simp: hp_prev.simps hp_prev_children.simps split: option.splits simp del: )
+  subgoal by auto
+  subgoal by auto
+  done
+
+lemma hp_child_hp_rescale_None_iff[simp]: \<open>hp_child a (hp_rescale_weight x1 x) = None \<longleftrightarrow>  hp_child a x = None\<close>
+  apply (induction x) 
+  subgoal for x xs children
+    apply (cases children)
+     apply (auto simp: hp_child.simps hp_child_children_def
+        List.map_filter_def option_hd_def filter_empty_conv split: option.splits)+
+    by fastforce
+  done
+
+lemma [simp]: \<open>map_option node (hp_child x (hp_rescale_weight x1 y)) = map_option node (hp_child x y)\<close>
+  apply (induction x y rule: hp_child.induct)
+  subgoal
+    by (auto simp: hp_child.simps split: option.splits simp del: )
+  subgoal by (auto simp: hp_child.simps split: option.splits)
+  done
+  
+lemma hp_parent_hp_rescale_None_iff[simp]: \<open>hp_parent a (hp_rescale_weight x1 x) = None \<longleftrightarrow>  hp_parent a x = None\<close>
+  apply (induction x) 
+  subgoal for x xs children
+    apply (cases children)
+    by (auto simp: hp_parent.simps hp_child_children_def
+        List.map_filter_def option_hd_def filter_empty_conv split: option.splits)+
+  done
+
+lemma ex_hp_parent_hp_rescale_weight[iff]: \<open>(\<exists>y. hp_parent n (hp_rescale_weight x1 x) = Some y) \<longleftrightarrow> (\<exists>y. hp_parent n (x) = Some y)\<close>
+  by (metis hp_parent_hp_rescale_None_iff not_None_eq2)
+
+lemma [simp]: \<open>map_option node (hp_parent x (hp_rescale_weight x1 y)) = map_option node (hp_parent x y)\<close>
+  apply (induction x y rule: hp_parent.induct)
+  subgoal for n a sc x children
+    apply (cases \<open> (filter (\<lambda>x. \<exists>y. hp_parent n x = Some y) children)\<close>)
+    apply (auto simp: hp_parent.simps filter_empty_conv filter_map comp_def)
+    apply force
+    by (metis (no_types, lifting) filter_eq_ConsD hp_parent_hp_rescale_None_iff in_list_in_setD option.map_sel)
+  subgoal by (auto simp: hp_parent.simps)
+  done
+
+lemma [simp]: \<open>map_option score (map_option (hp_rescale_weight x1) (hp_node x y)) = map_option (\<lambda>x. x div x1) (hp_score x y)\<close>
+  apply (induction x y rule: hp_node.induct)
+  subgoal by (auto simp:  split: option.splits)
+  subgoal by (auto simp: )
+  done
+
+lemma score_hp_rescale_weights_hp_node: \<open> v \<in># mset_nodes ya \<Longrightarrow>
+       score (the (map_option (hp_rescale_weight x1) (hp_node v ya))) =
+      (\<lambda>x. x div x1) ((the (hp_score v ya)))\<close>
+  by (metis hp.exhaust_sel hp.sel(2) hp_node_None_notin2 hp_rescale_weight.simps option.map_sel)
+
+(*hp_child, hp_parent, hp_score*)
+
+
+lemma encoded_hp_prop_list_conc_rescale_weights:
+  \<open> encoded_hp_prop_list_conc (ck, (cl, cm, cn, co, cp), cq) (cr, Some y) \<Longrightarrow>
+       encoded_hp_prop_list_conc
+        (ck, (cl, cm, cn, co, \<lambda>x. map_option (\<lambda>x. x div x1) (cp x)), cq)
+        (cr, Some (hp_rescale_weight x1 y))\<close>
+  by (auto simp: encoded_hp_prop_list_conc_def encoded_hp_prop_def)
+
+lemma mop_hp_decreases_weights_mop_prio_change_all_weights:
+  \<open>(uncurry (mop_hp_decreases_weights), uncurry (ACIDS.mop_prio_change_all_weights')) \<in> [\<lambda>(a, _). a > 0]\<^sub>f
+  nat_rel \<times>\<^sub>f acids_encoded_hmrel  \<rightarrow> \<langle>acids_encoded_hmrel\<rangle>nres_rel\<close>
+  unfolding  mop_hp_decreases_weights_def mop_prio_change_all_weights_alt_def
+     mop_hp_needs_rescaling_def uncurry_def ACIDS.mop_prio_change_all_weights'_def
+     mop_hp_decreases_weights_only_def
+  apply (intro frefI nres_relI)
+  apply refine_vcg
+  apply (auto simp: mop_hp_decreases_weights_def ACIDS.mop_prio_change_all_weights_def
+     mop_hp_needs_rescaling_def acids_encoded_hmrel_def intro!: RETURN_SPEC_refine)
+  apply (rule_tac x= \<open>\<lambda>x. dp x div x1\<close> in exI)
+  apply (rule_tac b= \<open>(dl, map_option (hp_rescale_weight x1) dm)\<close> in relcomp.relcompI)
+   apply (auto simp: mop_hp_decreases_weights_def ACIDS.mop_prio_change_all_weights_def ACIDS.hmrel_def
+     mop_hp_needs_rescaling_def acids_encoded_hmrel_def score_hp_rescale_weights_hp_node
+     intro!: RETURN_SPEC_refine
+     intro: encoded_hp_prop_list_conc_rescale_weights ACIDS.invar_hp_rescale_weight)
+    apply (auto simp: encoded_hp_prop_list_conc_def encoded_hp_prop_def simp add: option.map_sel)
+  done
+
+
 lemmas [sepref_fr_rules] =
   mop_hp_insert_impl_code.refine[FCOMP mop_hp_insert_impl_spec2, FCOMP hp_insert_spec_mop_prio_insert2]
   mop_rescale_and_reroot_code.refine[FCOMP mop_rescale_and_reroot_spec2, FCOMP rescale_and_reroot_mop_prio_change_weight2]
   mop_hp_is_in_code.refine[FCOMP mop_hp_is_in_spec2, FCOMP hp_is_in_mop_prio_is_in2]
   mop_vsids_pop_min2_impl_code.refine[FCOMP mop_vsids_pop_min2_impl2, FCOMP vsids_pop_min2_mop_prio_pop_min2]
   mop_hp_read_score_imp_code.refine[FCOMP mop_hp_read_score_imp_mop_hp_read_score2, FCOMP mop_hp_read_score_mop_prio_old_weight2]
+
+
+
+lemma mop_imp_decreases_weights_mop_hp_decreases_weights2:
+    \<open>(uncurry mop_imp_decreases_weights, uncurry (mop_hp_decreases_weights)) \<in>
+     [\<lambda>_. True]\<^sub>f nat_rel \<times>\<^sub>f (\<langle>\<langle>nat_rel\<rangle>option_rel, \<langle>nat_rel\<rangle>option_rel\<rangle>pairing_heaps_rel) \<rightarrow>
+     \<langle>\<langle>\<langle>nat_rel\<rangle>option_rel, \<langle>nat_rel\<rangle>option_rel\<rangle>pairing_heaps_rel\<rangle>nres_rel\<close>
+  unfolding uncurry_def
+  apply (intro nres_relI frefI)
+  subgoal for x y
+  apply (erule prod_relE)
+    apply hypsubst
+    unfolding split
+    apply (rule mop_imp_decreases_weights_mop_hp_decreases_weights)
+      apply auto
+    done
+  done
+
+
+lemmas [sepref_fr_rules] =
+  mop_imp_decrease_weights_code.refine[FCOMP mop_imp_decreases_weights_mop_hp_decreases_weights2,
+    FCOMP mop_hp_decreases_weights_mop_prio_change_all_weights,
+    unfolded acids_assn_def[symmetric]]
 
 end
